src/Implementations/Log/Log.v
@@ -45,6 +45,112 @@ Axiom decode_header : value -> header.
 Axiom encode_decode_header : forall hdr, decode_header (encode_header hdr) = hdr.
 Axiom decode_encode_header : forall v, encode_header (decode_header v) = v.
 
+
+
+(* Programs *)
+Local Definition read_header :=
+  hd <- |DO| Read hdr_block_num;
+  Ret (decode_header hd).
+
+Local Definition write_header hdr :=
+  _ <- |DO| Write hdr_block_num (encode_header hdr);
+  Ret tt.
+
+Local Definition apply_txn txn log_blocks :=
+  let key := txn_key txn in
+  let start := txn_start txn in
+  let addr_count := addr_count txn in
+  let data_count := data_count txn in
+  let txn_blocks := firstn (addr_count+data_count) (skipn start log_blocks) in
+  plain_blocks <- decrypt_all key txn_blocks;
+  let addr_blocks := firstn addr_count plain_blocks in
+  let data_blocks := skipn addr_count plain_blocks in
+  let addr_list := firstn data_count (blocks_to_addr_list addr_blocks)in
+  _ <- write_batch addr_list data_blocks;
+  Ret tt.
+
+Local Fixpoint apply_txns txns log_blocks :=
+  match txns with
+  | nil =>
+    Ret tt
+  | txn::txns' =>
+    _ <- apply_txn txn log_blocks;
+    _ <- apply_txns txns' log_blocks;
+    Ret tt  
+  end.
+
+Local Definition flush_txns txns log_blocks :=
+  _ <- apply_txns txns log_blocks;
+  _ <- write_header header0;
+  _ <- |DO| Sync;
+  Ret tt.
+
+Local Definition check_and_flush txns log hash :=
+  log_hash <- hash_all hash0 log;
+  if (hash_dec log_hash hash) then
+    _ <- flush_txns txns log;
+    Ret true
+  else
+    Ret false.
+
+Definition apply_log :=
+  hdr <- read_header;
+  let old_hash := old_hash hdr in
+  let old_count := old_count hdr in
+  let old_txn_count := old_txn_count hdr in  
+  let cur_hash := cur_hash hdr in
+  let cur_count := cur_count hdr in
+  let txns := txn_records hdr in
+  log <- read_consecutive log_start cur_count;
+  success <- check_and_flush txns log cur_hash;
+  if success then
+    Ret tt
+  else
+    let old_txns := firstn old_txn_count txns in
+    let old_log := firstn old_count log in
+    success <- check_and_flush old_txns old_log old_hash;
+    Ret tt.
+
+
+Local Definition commit_txn (addr_l data_l: list value) :=
+  hdr <- read_header;
+  let cur_hash := cur_hash hdr in
+  let cur_count := cur_count hdr in
+  let txns := txn_records hdr in
+  new_key <- |CO| GetKey (addr_l++data_l);
+  enc_data <- encrypt_all new_key (addr_l ++ data_l);
+  new_hash <- hash_all cur_hash enc_data;
+
+  _ <- write_consecutive (log_start + cur_count) enc_data;
+
+  let new_count := cur_count + (length addr_l + length data_l) in
+  let new_txn := Build_txn_record new_key cur_count (length addr_l) (length data_l) in
+  let new_hdr := Build_header cur_hash cur_count (length txns) new_hash new_count (txns++[new_txn]) in
+  _ <- write_header new_hdr;
+  _ <- |DO| Sync;
+  Ret tt.
+
+Definition commit (addr_l data_l: list value) :=
+  hdr <- read_header;
+  let cur_hash := cur_hash hdr in
+  let cur_count := cur_count hdr in
+  let txns := txn_records hdr in
+  let new_count := cur_count + (length addr_l + length data_l) in
+  _ <-
+  if (log_length <? new_count) then
+    apply_log 
+  else
+    Ret tt;
+  _ <- commit_txn addr_l data_l;
+  Ret tt.
+
+
+(* Representation Invariants *)
+
+Inductive Log_State :=
+| Synced : Log_State
+| Not_Synced : Log_State.
+
 Definition get_valid_part (hdr: header) blocks : header_part :=
   if (hash_dec (cur_hash hdr) (rolling_hash hash0 (firstn (cur_count hdr) blocks))) then
     Build_header_part (cur_hash hdr) (cur_count hdr) (txn_records hdr)
@@ -93,6 +199,7 @@ Definition hash_valid log_blocks hash :=
 Open Scope pred_scope.
 
 Definition log_rep_inner
+           (log_state: Log_State)
            (hdr: header) (txns: list txn)
            (hdr_blockset: set value) (log_blocksets: list (set value))
            (ax: list key * encryptionmap * hashmap) :=
@@ -107,6 +214,13 @@ Definition log_rep_inner
     (* Log Blocks *)
     log_start |=> log_blocksets *
     [[ hdr = decode_header (fst hdr_blockset)]] *
+    [[ match log_state with
+       | Synced =>
+         snd hdr_blockset = []
+       | Not_Synced =>
+         exists v, snd hdr_blockset = v :: nil
+       end
+    ]] *
     (* log length is valid *)
     [[ length log_blocksets = log_length ]] *
     (* txns represents the right thing *)
@@ -117,104 +231,9 @@ Definition log_rep_inner
     (* Header current txn_records are valid *)
     [[ txns_valid txns valid_log_blocks kl em ]].
 
-Definition log_rep (hdr: header) (txns: list txn) (ax: list key * encryptionmap * hashmap) :=
-  exists* (hdr_blockset: set value)(log_blocksets: list (set value)),
-    log_rep_inner hdr txns hdr_blockset log_blocksets ax.
+Definition log_rep (log_state: Log_State) (hdr: header) (txns: list txn) (ax: list key * encryptionmap * hashmap) :=
+  exists* (hdr_blockset: set value) (log_blocksets: list (set value)),
+    log_rep_inner log_state hdr txns hdr_blockset log_blocksets ax.
 
 Hint Extern 0 (okToUnify (log_rep_inner _ _ ?b _) (log_rep_inner _ _ ?b  _)) => constructor : okToUnify.
 Hint Extern 0 (okToUnify (log_rep ?txns _) (log_rep ?txns _)) => constructor : okToUnify.
-
-(* Programs *)
-Local Definition read_header :=
-  hd <- |DO| Read _ hdr_block_num;
-  Ret (decode_header hd).
-
-Local Definition write_header hdr :=
-  _ <- |DO| Write hdr_block_num (encode_header hdr);
-  Ret tt.
-
-Local Definition apply_txn txn log_blocks :=
-  let key := txn_key txn in
-  let start := txn_start txn in
-  let addr_count := addr_count txn in
-  let data_count := data_count txn in
-  let txn_blocks := firstn (addr_count+data_count) (skipn start log_blocks) in
-  plain_blocks <- decrypt_all key txn_blocks;
-  let addr_blocks := firstn addr_count plain_blocks in
-  let data_blocks := skipn addr_count plain_blocks in
-  let addr_list := firstn data_count (blocks_to_addr_list addr_blocks)in
-  _ <- write_batch addr_list data_blocks;
-  Ret tt.
-
-Local Fixpoint apply_txns txns log_blocks :=
-  match txns with
-  | nil =>
-    Ret tt
-  | txn::txns' =>
-    _ <- apply_txn txn log_blocks;
-    _ <- apply_txns txns' log_blocks;
-    Ret tt  
-  end.
-
-Local Definition flush_txns txns log_blocks :=
-  _ <- apply_txns txns log_blocks;
-  _ <- write_header header0;
-  Ret tt.
-
-Local Definition check_and_flush txns log hash :=
-  log_hash <- hash_all hash0 log;
-  if (hash_dec log_hash hash) then
-    _ <- flush_txns txns log;
-    Ret true
-  else
-    Ret false.
-
-Definition apply_log :=
-  hdr <- read_header;
-  let old_hash := old_hash hdr in
-  let old_count := old_count hdr in
-  let old_txn_count := old_txn_count hdr in  
-  let cur_hash := cur_hash hdr in
-  let cur_count := cur_count hdr in
-  let txns := txn_records hdr in
-  log <- read_consecutive log_start cur_count;
-  success <- check_and_flush txns log cur_hash;
-  if success then
-    Ret tt
-  else
-    let old_txns := firstn old_txn_count txns in
-    let old_log := firstn old_count log in
-    success <- check_and_flush old_txns old_log old_hash;
-    Ret tt.
-
-
-Local Definition commit_txn (addr_l data_l: list value) :=
-  hdr <- read_header;
-  let cur_hash := cur_hash hdr in
-  let cur_count := cur_count hdr in
-  let txns := txn_records hdr in
-  new_key <- |CO| GetKey (addr_l++data_l);
-  enc_data <- encrypt_all new_key (addr_l ++ data_l);
-  new_hash <- hash_all cur_hash enc_data;
-
-  _ <- write_consecutive (log_start + cur_count) enc_data;
-
-  let new_count := cur_count + (length addr_l + length data_l) in
-  let new_txn := Build_txn_record new_key cur_count (length addr_l) (length data_l) in
-  let new_hdr := Build_header cur_hash cur_count (length txns) new_hash new_count (txns++[new_txn]) in
-  _ <- write_header new_hdr;
-  Ret tt.
-
-Definition commit (addr_l data_l: list value) :=
-  hdr <- read_header;
-  let cur_hash := cur_hash hdr in
-  let cur_count := cur_count hdr in
-  let txns := txn_records hdr in
-  let new_count := cur_count + (length addr_l + length data_l) in
-  _ <-
-  if (new_count <=? log_length) then
-    apply_log 
-  else
-    Ret tt;
-  _ <- commit_txn addr_l data_l;
-  Ret tt.
