src/Refinements/LogCacheToLoggedDisk/Definitions.v
@@ -1,4 +1,4 @@
-Require Import Framework CachedDiskLayer LoggedDiskLayer LogCache.
+Require Import Framework CachedDiskLayer LoggedDiskLayer Log LogCache.
 Close Scope pred_scope.
 Import ListNotations.
 
@@ -7,37 +7,46 @@ Local Definition high_op := LoggedDiskOperation.
 Local Definition low := CachedDiskLang.
 Local Definition high := LoggedDiskLang.
 
-Definition compile_op T (p2: Operation.prog high_op T) : prog low T.
+Definition compile T (p2: Operation.prog high_op T) : prog low T.
  destruct p2.
  exact (read a).
  exact (write l l0).
 Defined.
 
-Definition oracle_refines_to_op T (d1: state low) (p: Operation.prog high_op T) o1 o2 : Prop :=
+Definition oracle_refines_to T (d1: state low) (p: Operation.prog high_op T) o1 o2 : Prop :=
    match p with
-     | Read a =>
-       (exists d1',
-          exec low o1 d1 (read a) (Crashed d1') /\
-          o2 = [CrashBefore]) \/
-       (exists d1' r,
-          exec low o1 d1 (read a) (Finished d1' r) /\
-          o2 = [Cont])
+   | Read a =>
+     (exists d1' r,
+        exec low o1 d1 (read a) (Finished d1' r) /\
+        o2 = [Cont] /\
+        d1' = d1) \/
+     (exists d1',
+        exec low o1 d1 (read a) (Crashed d1') /\
+        o2 = [CrashBefore] /\
+        d1 = d1')
          
-     | Write la lv =>
-       (exists d1',
-          exec low o1 d1 (write la lv) (Crashed d1') /\
-          ((d1' = d1 /\
-           o2 = [CrashBefore]) \/
-           (d1' <> d1 /\
-            o2 = [CrashAfter]))) \/
-       (exists d1' r,
+   | Write la lv =>
+     (exists d1' r,
           exec low o1 d1 (write la lv) (Finished d1' r) /\          
           o2 = [Cont] /\
-       (forall s ,(exists F, cached_log_rep F s d1) -> (exists F, cached_log_rep F (write_all s la lv) d1')))
+          (forall s,
+             (exists F log_state, cached_log_rep F s d1 log_state) ->
+             (exists F log_state, cached_log_rep F (write_all s la lv) d1' log_state))
+       ) \/
+     (exists d1',
+        (exec low o1 d1 (write la lv) (Crashed d1') /\
+         o2 = [CrashBefore] /\
+         d1' = d1) \/
+        (exec low o1 d1 (write la lv) (Crashed d1') /\
+         o2 = [CrashAfter] /\
+         d1' <> d1)
+     )  
    end.
 
   Definition refines_to (d1: state low) (d2: state high) :=
-    exists F, cached_log_rep F d2 d1.
+    exists F d2' log_state,
+      cached_log_rep F d2' d1 log_state /\
+      d2 = mem_map fst d2'.
 
-  Definition LoggedDiskOperationRefinement := Build_OperationRefinement compile_op refines_to oracle_refines_to_op.
+  Definition LoggedDiskOperationRefinement := Build_OperationRefinement compile refines_to oracle_refines_to.
   Definition LoggedDiskRefinement := LiftRefinement LoggedDiskLang LoggedDiskOperationRefinement.
