src/Refinements/LogCacheToLoggedDisk/LoggedDiskRefinement.v
@@ -1,1 +1,2 @@
-Require Export LogCacheToLoggedDisk.Definitions LogCacheToLoggedDisk.Refinement.
+Require Export LogCacheToLoggedDisk.Definitions.
+(* LogCacheToLoggedDisk.Refinement. *)
