src/Refinements/TransactionToTransactionalDisk/TransactionalDiskRefinement.v
@@ -1,1 +1,2 @@
-Require Export TransactionToTransactionalDisk.Definitions TransactionToTransactionalDisk.Refinement.
+Require Export TransactionToTransactionalDisk.Definitions.
+(* TransactionToTransactionalDisk.Refinement. *)
